---
title: 'DATA605: Fundamentals of Computational Mathematics'
author: "Donald Butler"
date: "05/07/2022"
output:
  pdf_document:
    extra_dependencies:
    - geometry
    - multicol
    - multirow
  word_document: default
subtitle: Discussion 14
---

```{r setup, include=FALSE}
knitr::opts_chunk$set(echo = TRUE)
```

## Chapter 8.8 Question 29

Use the Taylor series given in Key Idea 8.8.1 to find the first 4 terms of the Taylor series of the function $f(x) = e^x\sin(x)$.

$$e^x =\sum_{n=0}^{\infty}\frac{x^n}{n!} = 1 + x + \frac{x^2}{2!} + \frac{x^3}{3!} + \frac{x^4}{4!} + ...$$


$$\sin(x) = \sum_{n=0}^{\infty} (-1)^n \frac{x^{2n+1}}{(2n+1)!} = x - \frac{x^3}{3!} + ...$$

Multiplying term by term to find coefficients up to the $x^4$ term.

$$e^x \sin(x) = x - \frac{x^3}{3!} + x^2 - \frac{x^4}{3!} + \frac{x^3}{2!} + \frac{x^4}{3!}$$

Combining like terms we get:

$$e^x \sin(x) = x + x^2 + \frac{2x^3}{3!}$$

Another method for solving this problem would be to use the chain rule and calculate the first 4 derivatives.

$\begin{aligned}
f(x) & = e^x\sin(x) & \Rightarrow f(0) & = 0 \\
f'(x) & = e^x\cos(x) + e^x\sin(x) & \Rightarrow f'(0) & = 1 \\
f''(x) & = 2e^x\cos(x) & \Rightarrow f''(0) & = 2 \\
f'''(x) & = -2e^x\sin(x) + 2e^x\cos(x) & \Rightarrow f'''(0) & = 2 \\
f''''(x) & = -4e^x\sin(x) & \Rightarrow f''''(0) & = 0
\end{aligned}$

This gives us:

$$e^x \sin(x) = \frac{0}{0!} + \frac{1}{1!}x + \frac{2}{2!}x^2 + \frac{2}{3!}x^3 + \frac{0}{4!}x^4 = x + x^2 + \frac{2x^3}{3!}$$

